LambdaS5/coq/LjsCorrectness.v
@@ -1,0 +1,152 @@
+Set Implicit Arguments.
+Require Import LjsShared.
+Require Import Syntax.
+Require Import PrettyInterm.
+Require Import PrettyRules.
+Require Import Store.
+Require Import Context.
+Require Import Values.
+Require Import Operators.
+Require Import Monads.
+Require Import Interpreter.
+Require Import Coq.Strings.String.
+
+Require Import List.
+Import ListNotations.
+
+Open Scope list_scope.
+
+Implicit Type A B : Type.
+Implicit Type st : store.
+Implicit Type e : expr.
+Implicit Type v : value.
+Implicit Type loc : value_loc.
+Implicit Type s : string.
+Implicit Type n : number.
+Implicit Type i : id.
+Implicit Type o : out.
+Implicit Type c : ctx.
+Implicit Type ptr : object_ptr.
+Implicit Type obj : object.
+Implicit Type re : result.
+Implicit Type r : res.
+
+Record runs_type_correct runs :=
+    make_runs_type_correct {
+        runs_type_correct_eval : forall c st e o,
+            runs_type_eval runs c st e = result_some o -> red_expr c st e o
+}.
+
+(* Lemmas on monadic ops *)
+
+Definition is_some {A} ra (Pred : A -> Prop) :=
+    exists a, ra = result_some a /\ Pred a.
+
+Hint Unfold is_some.
+
+Lemma is_some_covariant : forall A (P1 P2 : A -> Prop), 
+    (forall a, P1 a -> P2 a) -> 
+    forall ra, is_some ra P1 -> is_some ra P2. 
+Proof. unfold is_some. jauto. Qed.
+
+Hint Resolve is_some_covariant.
+
+Lemma if_result_some_out : forall A B (ra : resultof A) (b : B) cont, 
+    if_result_some ra cont = result_some b -> 
+    is_some ra (fun a => cont a = result_some b).
+Proof. introv E. destruct* ra; intros; false. Qed.
+
+Definition if_out_ter_post (cont : store -> res -> result) o' o :=
+    (exists st r, o = out_ter st r /\ cont st r = result_some o') \/
+    (o = out_div /\ o' = o).
+
+Lemma if_out_ter_out : forall re o cont, 
+    if_out_ter re cont = result_some o -> 
+    is_some re (if_out_ter_post cont o).
+Proof.
+    introv E.
+    lets H: if_result_some_out E.
+    gen H. 
+    apply is_some_covariant.
+    intros o1 E1.  
+    destruct o1; inverts E1; unfolds*; tryfalse.
+Qed.
+
+Definition eqabort o' o := abort o /\ o' = o.
+
+Hint Unfold eqabort.
+
+Definition if_value_post (cont : store -> value -> result) o' o := 
+    (exists st v, o = out_ter st (res_value v) /\ cont st v = result_some o') \/
+    eqabort o' o.
+
+Lemma if_value_out : forall re o cont,
+    if_value re cont = result_some o ->
+    is_some re (if_value_post cont o).
+Proof.
+    introv E. 
+    apply if_out_ter_out in E. 
+    gen E.
+    apply is_some_covariant.
+    intros o1 E.
+    unfolds.
+    destruct o1;
+    (inverts E as H; [inverts H as H; inverts H as H; inverts H as H H1 | inverts H as H]); jauto; tryfalse.
+    destruct* x0; inverts H; inverts H1; jauto.
+Qed.
+
+Lemma assert_get_object_ptr_out : forall v o cont,
+    assert_get_object_ptr v cont = result_some o ->
+    exists ptr, v = value_object ptr /\ cont ptr = result_some o.
+Proof.
+    introv E. destruct* v; false.
+Qed.
+
+Lemma assert_get_string : forall v o cont,
+    assert_get_string v cont = result_some o ->
+    exists s, v = value_string s /\ cont s = result_some o.
+Proof.
+    introv E. destruct* v; false.
+Qed.
+
+Lemma assert_get_bool : forall v o cont,
+    assert_get_bool v cont = result_some o ->
+    exists b, v = bool_to_value b /\ cont b = result_some o.
+Proof.
+    introv E. destruct* v; tryfalse; [exists true | exists false]; jauto. 
+Qed.
+
+Lemma assert_get_object_from_ptr_out : forall st ptr o cont,
+    assert_get_object_from_ptr st ptr cont = result_some o ->
+    exists obj, get_object st ptr = Some obj /\ cont obj = result_some o.
+Proof.
+    introv E. unfold assert_get_object_from_ptr in E.
+    destruct* (get_object st ptr); tryfalse.
+Qed.
+
+Lemma assert_get_object_out : forall st v o cont,
+    assert_get_object st v cont = result_some o -> 
+    exists ptr obj, v = value_object ptr /\ get_object st ptr = Some obj /\ cont obj = result_some o.
+Proof. 
+    introv E. 
+    unfold assert_get_object in E.
+    lets (ptr&Hptr&Cptr): assert_get_object_ptr_out E.
+    lets (obj&Hobj&Cobj): assert_get_object_from_ptr_out Cptr.
+    jauto.
+Qed.
+
+Lemma assert_some_out : forall A opt cont (o : option A),
+    assert_some opt cont = result_some o ->
+    exists (a : A), opt = Some a /\ cont a = result_some o.
+Proof. 
+    introv E.
+    destruct* opt; tryfalse.
+Qed.
+
+Lemma assert_deref_out : forall st loc cont o,
+    assert_deref st loc cont = result_some o ->
+    exists v, get_value st loc = Some v /\ cont v = result_some o.
+Proof.
+    introv E. unfold assert_deref in E.
+    destruct* (get_value st loc); tryfalse.
+Qed.
