LambdaS5/coq/LjsShared.v
@@ -1,0 +1,5 @@
+Set Implicit Arguments.
+Require Export LibTactics LibCore LibString LibFset LibSet.
+Generalizable Variables A B.
+Require Export LibProd LibListZ.
+
